stlc/lngen/def_ltac.v
@@ -1,0 +1,169 @@
+Require Import Coq.Program.Equality.
+Require Export Metalib.Metatheory.
+
+Require Import stlc.lngen.def_ott.
+Require Import stlc.lngen.def_extra.
+
+Ltac inst_cofinite_impl H x :=
+  match type of H with
+    | forall x, x `notin` ?L -> _ =>
+        let Fr := fresh "Fr" in
+          assert (x `notin` L) as Fr by auto;
+        specialize (H x Fr); clear Fr
+  end.
+
+Ltac inst_cofinites_with x :=
+  repeat
+    match goal with
+      | H : forall x0, x0 `notin` ?L -> _ |- _ =>
+          inst_cofinite_impl H x
+    end.
+
+Ltac inst_cofinite_impl_keep H x :=
+  match type of H with
+    | forall x, x `notin` ?L -> _ =>
+      let H_1 := fresh "H" in
+        let Fr := fresh "Fr" in
+          assert (x `notin` L) as Fr by auto;
+          specialize (H x Fr) as H_1; generalize dependent H
+  end.
+
+  
+Ltac inst_cofinites_with_keep x :=
+  repeat
+    match goal with
+      | H : forall x0, x0 `notin` ?L -> _ |- _ =>
+          inst_cofinite_impl_keep H x
+    end;
+  intros.
+
+Tactic Notation "inst_cofinites_with" ident(x) := 
+  inst_cofinites_with x.
+
+Tactic Notation "inst_cofinites_with" ident(x) "(keep)" := 
+  inst_cofinites_with_keep x.
+
+Ltac inst_cofinites :=
+  match goal with
+  | x : atom |- _ => inst_cofinites_with x
+  end.
+
+Ltac inst_cofinites_with_new :=
+  let x := fresh "x" in
+  pick fresh x; inst_cofinites_with x.
+
+Ltac inst_cofinites_by F :=
+  let L := F in
+  let x := fresh "x" in
+  pick fresh x for L; inst_cofinites_with x.
+  
+Tactic Notation "inst_cofinites_by" constr(F) :=
+  let x := fresh "x" in let L:=F in pick fresh x for L; inst_cofinites_with x.
+Tactic Notation "inst_cofinites_by" constr(L) "using_name" ident(x) := 
+  let x := fresh x in pick fresh x for L; inst_cofinites_with x.
+
+Ltac solve_notin_eq X :=
+  let H := fresh "H" in
+    assert (H: X `notin` singleton X) by auto;
+    apply notin_singleton_1 in H; contradiction.
+
+  
+Ltac destruct_eq_atom :=
+  unfold eq_dec in *;
+  repeat
+    lazymatch goal with
+    | H : context [EqDec_eq_of_X ?X ?X] |- _ => destruct (EqDec_eq_of_X X X); [ idtac | contradiction]
+    | H : _ |- context [EqDec_eq_of_X ?X ?X] => destruct (EqDec_eq_of_X X X); [ idtac | contradiction]
+    | H : context [EqDec_eq_of_X ?X0 ?X] |- _ => destruct (EqDec_eq_of_X X0 X); subst;
+        try contradiction; try solve_notin_eq X0; try solve_notin_eq X
+    | H : _ |- context [EqDec_eq_of_X ?X0 ?X] => destruct (EqDec_eq_of_X X0 X); subst;
+        try contradiction; try solve_notin_eq X0; try solve_notin_eq X
+    end.
+
+Ltac auto_apply :=
+  match goal with
+  | H : context [ ?P -> ?Q ] |- ?Q => apply H
+  end.
+
+Ltac gather_atoms ::=
+  let A := gather_atoms_with (fun x : vars => x) in
+  let B := gather_atoms_with (fun x : var => {{ x }}) in
+  let C := gather_atoms_with (fun x => var_in_exp x) in
+  let D := gather_atoms_with (fun x : ctx => dom x) in
+
+  constr:(A \u B \u C \u D).
+
+Tactic Notation "inst_cofinites_for" constr(H) := 
+  let L1 := gather_atoms in
+  let L1 := beautify_fset L1 in
+  apply H with (L:=L1).
+
+Tactic Notation "inst_cofinites_for" constr(H) ident(name)":="constr(Args1) := 
+  let L1 := gather_atoms in
+  let L1 := beautify_fset L1 in
+  apply H with (L:=L1) (name:=Args1).
+
+Tactic Notation "inst_cofinites_for" constr(H) ident(argname1)":="constr(arg1) "," ident(argname2) ":=" constr(arg2):= 
+  let L1 := gather_atoms in
+  let L1 := beautify_fset L1 in
+  apply H with (L:=L1) (argname1:=arg1) (argname2:=arg2).
+
+Tactic Notation "inst_cofinites_for" constr(H) ident(argname1)":="constr(arg1) "," ident(argname2) ":=" constr(arg2)"," ident(argname3) ":=" constr(arg3):= 
+  let L1 := gather_atoms in
+  let L1 := beautify_fset L1 in
+  apply H with (L:=L1) (argname1:=arg1) (argname2:=arg2)  (argname3:=arg3).
+
+(* destruct conjunctions *)
+Ltac destruct_conj :=
+  repeat match goal with H: ?T |- _ =>
+                         lazymatch T with
+                         | exists _ , _ => destruct H
+                         | _ /\ _ => destruct H
+                         end
+    end.
+
+Ltac solve_by_inverts n :=
+  match goal with | H : ?T |- _ =>
+  match type of T with Prop =>
+    solve [
+      inversion H;
+      match n with S (S (?n')) => subst; solve_by_inverts (S n') end ]
+  end end.
+
+Ltac solve_by_invert :=
+  solve_by_inverts 1.
+
+Ltac destruct_binds_eq :=
+  repeat
+    lazymatch goal with
+    | H1 : (?X1, ?b1) = (?X2, ?b2) |- _ =>
+      dependent destruction H1
+    end.
+
+Ltac destruct_binds :=
+  simpl in *;
+  repeat
+  match goal with
+  | H1 : binds ?X ?b ((?X', ?b') :: ?θ) |- _ =>
+    let H_1 := fresh "H" in
+    let H_2 := fresh "H" in
+    inversion H1 as [H_1 | H_2];
+    clear H1;
+    try destruct_binds_eq;
+    try solve [solve_notin_eq X];
+    try solve [solve_notin_eq X']
+  end.
+
+Ltac destruct_in :=
+  simpl in *;
+  match goal with
+  | H1 : ((?X, ?b) = (?X', ?b')) \/  In ?b'' ?θ |- _ =>
+    let H1_1 := fresh "H" in
+    let H1_2 := fresh "H" in
+    inversion H1 as [H1_1 | H1_2];
+    clear H1;
+    try destruct_binds_eq;
+    try solve [solve_notin_eq X];
+    try solve [solve_notin_eq X']
+  end.
+                                
