stlc/lngen/prop_typing.v
@@ -3,8 +3,38 @@ Require Import stlc.lngen.prop_ln.
 Require Import stlc.lngen.def_extra.
 
 Require Import Coq.Program.Equality.
+Require Import Metalib.Metatheory.
+
+Require Import stlc.lngen.def_ltac.
 
 Hint Constructors typing : core.
+
+Lemma typing_lc Γ t A : 
+  Γ ⊢ t : A ->
+  lc_exp t.
+Proof.
+  intros. induction H; eauto.
+Qed.
+
+Lemma binds_same {T} Γ1 Γ2 x (A B : T): 
+  binds x A (Γ2 ++ (x, B) :: Γ1) ->
+  x `notin` dom (Γ2 ++ Γ1) ->
+  A = B.
+Proof.
+  intros. induction Γ2; destruct_binds; eauto.
+  - exfalso. eapply binds_dom_contradiction; eauto.
+  - destruct a. destruct_binds; eauto.
+Qed.
+
+Lemma typing_weaken Γ1 Γ2 Γ3 t A:
+  Γ3 ++ Γ1 ⊢ t : A ->
+  Γ3 ++ Γ2 ++ Γ1 ⊢ t : A.
+Proof.
+  intros. dependent induction H; eauto.
+  - inst_cofinites_for typing_abs. intros.
+    rewrite_env (((x, A) :: Γ3) ++ Γ2 ++ Γ1).
+    eapply H0; eauto.
+Qed.
 
 Theorem typing_subst Γ1 Γ2 x s t A B:
   x `notin` dom (Γ2 ++ Γ1) ->
@@ -13,12 +43,23 @@ Theorem typing_subst Γ1 Γ2 x s t A B:
   Γ2 ++ Γ1 ⊢ (subst_exp_in_exp s x t) : A.
 Proof.
   intros. dependent induction H0; eauto.
-  - simpl. destruct (x0 == x). admit.
-  - admit.
+  - simpl. destruct_eq_atom. eauto.
+    + eapply binds_same in H0; subst; eauto.
+      rewrite_env (nil ++ Γ2 ++ Γ1). eapply typing_weaken; eauto.
+    + apply binds_remove_mid in H0; eauto. 
+  - simpl. inst_cofinites_for typing_abs. intros.
+    inst_cofinites_with x0.
+    rewrite_env (((x0, A) :: Γ2) ++ Γ1). 
+    replace (exp_var_f x0) with (subst_exp_in_exp s x (exp_var_f x0)); eauto.
+    rewrite <- subst_exp_in_exp_open_exp_wrt_exp.
+    eapply H0; simpl; eauto.
+    + eapply typing_lc; eauto.
+    + simpl. destruct_eq_atom; eauto.
   - simpl. eapply typing_app; eauto.
-Admitted.
+Qed.
 
 Corollary typing_subst0 Γ x s t A B: 
+  x `notin` dom Γ ->
   ((x, B) :: Γ) ⊢ t : A ->
   Γ ⊢ s : B ->
   Γ ⊢ (subst_exp_in_exp s x t) : A.
@@ -33,5 +74,11 @@ Theorem preservation Γ t t' A :
 Proof.
   intros Htyping Hstep. generalize dependent A.
   induction Hstep; intros; inversion Htyping; subst; eauto.
-  - inversion H2. subst. admit.
-Admitted.
+  - inversion H2. subst.
+    pick fresh x. inst_cofinites_with x.
+    apply typing_subst0 with (s:=s) in H3; eauto.
+    rewrite subst_exp_in_exp_open_exp_wrt_exp in H3; eauto.
+    simpl in H3. destruct_eq_atom. eauto.
+    rewrite subst_exp_in_exp_fresh_eq in H3; eauto.
+    eapply typing_lc; eauto.
+Qed.
